- update notation - reorg ltac

proof/old_system/uni/algo_worklist/prop_basic.v
@@ -49,6 +49,7 @@ Proof.
 Qed.
  *)
 
+Hint Constructors a_wf_wl : Hdb_a_wl_red_basic.
 Hint Constructors a_wl_red : Hdb_a_wl_red_basic.
 Hint Constructors apply_cont : Hdb_a_wl_red_basic.
 Hint Constructors aworklist_subst : Hdb_a_wl_red_basic.
@@ -62,10 +63,10 @@ Proof.
   intros. induction H; simpl; try solve [simpl; eauto with Hdb_a_wl_red_basic].
 Qed.
 
-Fixpoint subst_tvar_in_etvar_list (X' X: typvar) (E:list typvar) :=
+Fixpoint rename_tvar_in_etvar_list (X' X: typvar) (E:list typvar) :=
   match E with 
   | nil => nil
-  | X0 :: E' => (if X0 == X then X' else X0) :: (subst_tvar_in_etvar_list X X' E') 
+  | X0 :: E' => (if X0 == X then X' else X0) :: (rename_tvar_in_etvar_list X' X E') 
   end.
 
 
@@ -80,23 +81,52 @@ end.
 Lemma worklist_subst_rename : forall Γ X X' A E Γ1 Γ2,
   aworklist_subst Γ X A E Γ1 Γ2 -> 
   aworklist_subst (rename_tvar_in_aworklist X' X Γ) X' ({` X' /ᵗ X} A) 
-      (subst_tvar_in_etvar_list X' X E) (rename_tvar_in_aworklist X' X Γ1) (rename_tvar_in_aworklist X' X Γ2).
+      (rename_tvar_in_etvar_list X' X E) (rename_tvar_in_aworklist X' X Γ1) (rename_tvar_in_aworklist X' X Γ2).
 Proof with auto with Hdb_a_wl_red_basic.
   intros. induction H; try solve [simpl; eauto with Hdb_a_wl_red_basic].
   - simpl. destruct (X == X)...
     contradiction.
-  - admit.
-  - 
+  - simpl in *. unfold eq_dec. 
+    destruct (EqDec_eq_of_X Y X). 
+    + subst. econstructor; auto. admit.
+    + constructor; auto. admit.
+  - simpl in *. unfold eq_dec. 
+    destruct (EqDec_eq_of_X Y X). 
+    + subst. econstructor; auto. admit.
+    + constructor; auto. admit.
+  - simpl in *. unfold eq_dec. 
+    destruct (EqDec_eq_of_X Y X). 
+    + subst. econstructor; auto. admit.
+    + constructor; auto. admit.
 Admitted.
 
 Lemma worklist_subst_rename' : forall Γ X1 X2 X' A E Γ1 Γ2,
   aworklist_subst Γ X2 A E Γ1 Γ2 -> 
   aworklist_subst (rename_tvar_in_aworklist X' X1 Γ) (if X2 == X1 then X' else X2) ({` X' /ᵗ X1} A) 
-      (subst_tvar_in_etvar_list X' X1 E) (rename_tvar_in_aworklist X' X1 Γ1) (rename_tvar_in_aworklist X' X1 Γ2).
+      (rename_tvar_in_etvar_list X' X1 E) (rename_tvar_in_aworklist X' X1 Γ1) (rename_tvar_in_aworklist X' X1 Γ2).
 Proof with auto with Hdb_a_wl_red_basic.
   intros. induction H; try solve [simpl; eauto with Hdb_a_wl_red_basic].
 Admitted.
 
+
+Lemma binds_var_typ_rename : forall x A X X' Γ,
+  ⊢ᵃ Γ ->
+  binds x (abind_var_typ A) (awl_to_aenv Γ) -> 
+  binds x (abind_var_typ ({` X' /ᵗ X} A)) (awl_to_aenv (rename_tvar_in_aworklist X' X Γ)).
+Proof with auto with Hdb_a_wl_red_basic.
+  intros. induction Γ.
+  - simpl in *. inversion H0.
+  - simpl in *. inversion H0.
+    + dependent destruction H1.
+      simpl. constructor... 
+    + apply binds_cons...
+      dependent destruction H...
+  - simpl in *. inversion H0.
+    + dependent destruction H1.
+      inversion H. 
+    + dependent destruction H; apply binds_cons...
+  - dependent destruction H. simpl in *...
+Qed.
 
 Theorem a_wl_red_rename_tvar : forall Γ X X',
   Γ ⟶ᵃʷ⁎⋅ ->
@@ -138,7 +168,7 @@ Proof with eauto with Hdb_a_wl_red_basic.
   - simpl. destruct (X0 == X).
     + subst.
       apply worklist_subst_rename with (X':=X') in H1 as Hsubst.
-      apply a_wl_red__sub_etvarmono1 with (E:=subst_tvar_in_etvar_list X' X E)
+      apply a_wl_red__sub_etvarmono1 with (E:=rename_tvar_in_etvar_list X' X E)
         (Γ1:=rename_tvar_in_aworklist X' X Γ1) (Γ2:=rename_tvar_in_aworklist X' X Γ2)
       ; auto... admit.
       admit.
@@ -168,7 +198,7 @@ Proof with eauto with Hdb_a_wl_red_basic.
     rewrite subst_tvar_in_exp_open_exp_wrt_exp in H0...
   - simpl in *.
     eapply a_wl_red__inf_var with (A:=({` X' /ᵗ X} A))...
-    admit.
+    apply binds_var_typ_rename... admit.
   - simpl in *.
     eapply a_wl_red__inf_tabs with (L:=L `union` singleton X)...
     intros. inst_cofinites_with X0.
@@ -181,11 +211,164 @@ Proof with eauto with Hdb_a_wl_red_basic.
   - simpl in *.  
     eapply a_wl_red__inf_abs_mono.
     admit.
-  - admit.
+  - simpl in *. 
+    eapply a_wl_red__infabs_all with (L:=L `union` singleton X)...
+    intros. inst_cofinites_with X0.
+    rewrite typ_subst_open_comm...
+    unfold eq_dec in H0.
+    destruct (EqDec_eq_of_X X0 X) in H0...
+    + subst. apply notin_union_2 in H1. apply notin_singleton_1 in H1. contradiction.
   - admit.
   - simpl in *. 
     eapply a_wl_red__inftapp_all.
     rewrite <- subst_tvar_in_typ_open_typ_wrt_typ...
   - simpl. 
     eapply apply_cont_rename with (X:=X) (X':=X') in H...
+Admitted.
+
+
+Ltac destruct_a_wf_wl :=
+  repeat
+    lazymatch goal with
+    | H : a_wf_wl (aworklist_conswork ?Γ ?w) |- _ => dependent destruction H
+    | H : a_wf_wl (aworklist_consvar ?Γ ?w ?b) |- _ => dependent destruction H
+    | H : a_wf_wl (aworklist_constvar ?Γ ?X ?b) |- _ => dependent destruction H
+    | H : a_wf_work ?Ω ?w |- _ => dependent destruction H
+    | H : a_wf_typ ?E (open_typ_wrt_typ ?A ?T) |- _ => fail
+    | H : a_wf_typ ?E (?Ct ?A1 ?A2) |- _ => dependent destruction H
+    | H : a_wf_exp ?E (?Ce ?b) |- _ => dependent destruction H
+    | H : a_wf_exp ?E (?Ce ?e1 ?e2) |- _ => dependent destruction H
+    | H : a_wf_cont ?E (?C_C _) |- _ => dependent destruction H
+    | H : a_wf_cont ?E (?C_C _ _) |- _ => dependent destruction H
+    | H : a_wf_cont ?E (?C_C _ _ _) |- _ => dependent destruction H
+    end.
+
+
+
+Ltac _apply_IH_a_wl_red :=
+  let H := fresh "H" in
+    match goal with 
+    | H : (⊢ᵃ ?Γ) -> ?P |- _ => destruct_a_wf_wl; 
+      let H1 := fresh "H" in
+      assert (H1 : ⊢ᵃ Γ) by auto with Hdb_a_wl_red_basic;
+      let H2 := fresh "IHHdred" in
+      apply H in H1 as H2
+    end.
+
+
+Theorem a_wl_red_rename_tvar' : forall Γ X X',
+  ⊢ᵃ Γ -> 
+  Γ ⟶ᵃʷ⁎⋅ ->
+  (rename_tvar_in_aworklist X' X Γ) ⟶ᵃʷ⁎⋅.
+Proof with eauto with Hdb_a_wl_red_basic.
+  intros. dependent induction H0; try solve [simpl; try _apply_IH_a_wl_red; eauto with Hdb_a_wl_red_basic].
+  - admit.
+  - simpl.
+    dependent destruction H.
+    eapply a_wl_red__sub_alll with (L:=L `union` singleton X).
+    + admit.
+    + admit.
+    + admit.
+    + intros. simpl in *. inst_cofinites_with X0.
+      assert (⊢ᵃ (work_sub (B1 ^ᵈ X0) A1 ⫤ aworklist_constvar Γ X0 abind_etvar_empty)) by admit. 
+      rewrite typ_subst_open_comm...
+      unfold eq_dec in H5.
+      destruct (EqDec_eq_of_X X0 X) in H5...
+      admit.
+  - simpl.
+    eapply a_wl_red__sub_all with (L:=L `union` singleton X).
+    intros. inst_cofinites_with X0.
+    simpl in H0.
+    rewrite typ_subst_open_comm...
+    rewrite typ_subst_open_comm...
+    admit.
+  - simpl. 
+    destruct (X0 == X).
+    + subst.
+      eapply a_wl_red__sub_arrow1 with (L:=L)... admit.
+      admit.
+      intros.
+      inst_cofinites_with X1. inst_cofinites_with X2.
+      admit.
+    + eapply a_wl_red__sub_arrow1 with (L:=L)... admit.
+      admit.
+      intros.
+      inst_cofinites_with X1. inst_cofinites_with X2.
+      admit.
+  - admit.
+  - simpl. destruct (X0 == X).
+    + subst.
+      apply worklist_subst_rename with (X':=X') in H2 as Hsubst.
+      apply a_wl_red__sub_etvarmono1 with (E:=rename_tvar_in_etvar_list X' X E)
+        (Γ1:=rename_tvar_in_aworklist X' X Γ1) (Γ2:=rename_tvar_in_aworklist X' X Γ2)
+      ; auto... admit.
+      admit.
+      admit.
+    + eapply a_wl_red__sub_etvarmono1; auto. admit.
+      admit.
+      admit.
+      admit.
+  - simpl. 
+    eapply worklist_subst_rename' with (X1:=X) (X':=X') in H2 as Hsubst.
+  destruct (X0 == X).
+    + subst.
+      eapply a_wl_red__sub_etvarmono2; auto. admit.
+       admit.
+       admit.
+       admit.
+    + eapply a_wl_red__sub_etvarmono2; auto. admit.
+      admit.
+      admit.
+      admit.
+  - simpl in *. 
+    eapply a_wl_red__chk_absarrow with (L:=L). intros.
+    inst_cofinites_with x.
+    assert (⊢ᵃ (work_check (open_exp_wrt_exp e (exp_var_f x)) A2 ⫤ aworklist_consvar Γ x (abind_var_typ A1))) by admit.
+    apply H1 in H3.
+    rewrite subst_tvar_in_exp_open_exp_wrt_exp in H3...
+  - admit.
+  - simpl in *. 
+    eapply a_wl_red__chk_abstop with (L:=L). intros.
+    inst_cofinites_with x.
+    assert (⊢ᵃ (work_check (open_exp_wrt_exp e (exp_var_f x)) typ_top ⫤ aworklist_consvar Γ x (abind_var_typ typ_bot))) by admit.
+    apply H1 in H3.
+    rewrite subst_tvar_in_exp_open_exp_wrt_exp in H3...
+  - simpl in *.
+    assert (⊢ᵃ (work_apply c A ⫤ Γ)) by admit.
+    dependent destruction H.
+    apply IHa_wl_red in H3.
+    eapply a_wl_red__inf_var with (A:=({` X' /ᵗ X} A))...
+    apply binds_var_typ_rename...
+  - simpl in *.
+    eapply a_wl_red__inf_tabs with (L:=L `union` singleton X)...
+    intros. inst_cofinites_with X0.
+    assert (⊢ᵃ (work_check (open_exp_wrt_typ e ` X0) (A ^ᵈ X0) ⫤ X0 ~ᵃ □ ;ᵃ work_apply c (typ_all A) ⫤ Γ)) by admit.
+    apply H1 in H3.
+    rewrite subst_tvar_in_exp_open_exp_wrt_typ in H3...
+    simpl in H3.
+    rewrite <- typ_subst_open_comm in H3...
+    unfold eq_dec in H3.
+    destruct (EqDec_eq_of_X X0 X) in H3...
+    + subst. apply notin_union_2 in H2. apply notin_singleton_1 in H2. contradiction.
+  - simpl in *.  
+    eapply a_wl_red__inf_abs_mono.
+    admit.
+  - simpl in *. 
+    eapply a_wl_red__infabs_all with (L:=L `union` singleton X)...
+    intros. inst_cofinites_with X0.
+    rewrite typ_subst_open_comm...
+    unfold eq_dec in H0.
+    destruct (EqDec_eq_of_X X0 X) in H0...
+    + subst. apply notin_union_2 in H2. apply notin_singleton_1 in H2. contradiction.
+    + admit.
+  - admit.
+  - simpl in *. 
+    assert ( ⊢ᵃ (work_apply c (A ^^ᵈ B) ⫤ Γ)) by admit.
+    apply IHa_wl_red in H1.
+    eapply a_wl_red__inftapp_all.
+    rewrite <- subst_tvar_in_typ_open_typ_wrt_typ...
+  - simpl. 
+    assert (⊢ᵃ (w ⫤ Γ)) by admit.
+    apply IHa_wl_red in H2.
+    eapply apply_cont_rename with (X:=X) (X':=X') in H0...
 Admitted.
